proofs/hol_light/aarch64/proofs/dump_bytecode.ml
@@ -14,6 +14,18 @@ print_string "=== bytecode start: aarch64/mldsa/mldsa_pointwise.o ===\n";;
 print_literal_from_elf "aarch64/mldsa/mldsa_pointwise.o";;
 print_string "==== bytecode end =====================================\n\n";;
 
+print_string "=== bytecode start: aarch64/mldsa/mldsa_pointwise_acc_l4.o ===\n";;
+print_literal_from_elf "aarch64/mldsa/mldsa_pointwise_acc_l4.o";;
+print_string "==== bytecode end =====================================\n\n";;
+
+print_string "=== bytecode start: aarch64/mldsa/mldsa_pointwise_acc_l5.o ===\n";;
+print_literal_from_elf "aarch64/mldsa/mldsa_pointwise_acc_l5.o";;
+print_string "==== bytecode end =====================================\n\n";;
+
+print_string "=== bytecode start: aarch64/mldsa/mldsa_pointwise_acc_l7.o ===\n";;
+print_literal_from_elf "aarch64/mldsa/mldsa_pointwise_acc_l7.o";;
+print_string "==== bytecode end =====================================\n\n";;
+
 print_string "=== bytecode start: aarch64/mldsa/mldsa_poly_caddq.o ===\n";;
 print_literal_from_elf "aarch64/mldsa/mldsa_poly_caddq.o";;
 print_string "==== bytecode end =====================================\n\n";;
