proofs/hol_light/x86_64/proofs/dump_bytecode.ml
@@ -16,3 +16,15 @@ print_string "==== bytecode end =====================================\n\n";;
 print_string "=== bytecode start: x86_64/mldsa/mldsa_pointwise.o ================\n";;
 print_literal_from_elf "x86_64/mldsa/mldsa_pointwise.o";;
 print_string "==== bytecode end =====================================\n\n";;
+
+print_string "=== bytecode start: x86_64/mldsa/mldsa_pointwise_acc_l4.o ================\n";;
+print_literal_from_elf "x86_64/mldsa/mldsa_pointwise_acc_l4.o";;
+print_string "==== bytecode end =====================================\n\n";;
+
+print_string "=== bytecode start: x86_64/mldsa/mldsa_pointwise_acc_l5.o ================\n";;
+print_literal_from_elf "x86_64/mldsa/mldsa_pointwise_acc_l5.o";;
+print_string "==== bytecode end =====================================\n\n";;
+
+print_string "=== bytecode start: x86_64/mldsa/mldsa_pointwise_acc_l7.o ================\n";;
+print_literal_from_elf "x86_64/mldsa/mldsa_pointwise_acc_l7.o";;
+print_string "==== bytecode end =====================================\n\n";;
